---
title: "TexText"
collection: publications
permalink: /:collection/textest
excerpt: "Tex表記のテスト"
date: 9999-12-31
venue:
paperurl:
citation:
---


## 1. test
```
$$
    y = ax + b \\
    \alpha \alpha = \beta + \gamma
$$
```
↓↓↓

$$
    y = ax + b \\
    \alpha \alpha = \beta + \gamma
$$


## 2. aligned
```
$$
    \begin{aligned}
        y &= ax + b \\
        \alpha \alpha &= \beta + \gamma
    \end{aligned}
$$
```
↓↓↓

$$
    \begin{aligned}
        y &= ax + b \\
        \alpha \alpha &= \beta + \gamma
    \end{aligned}
$$

## 3. aligned
```
\begin{aligned}
    y &= ax + b \\\\\\\\
    \alpha \alpha &= \beta + \gamma
\end{aligned}
```
↓↓↓

\begin{aligned}
    y &= ax + b \\\\\\\\
    \alpha \alpha &= \beta + \gamma
\end{aligned}


## 4. align
```
$$
    \begin{align}
        y &= ax + b \\
        \alpha \alpha &= \beta + \gamma
    \end{align}
$$
```
↓↓↓

$$
    \begin{align}
        y &= ax + b \\
        \alpha \alpha &= \beta + \gamma
    \end{align}
$$

## 5. align
```
\begin{align}
    y &= ax + b \\\\\\\\
    \alpha \alpha &= \beta + \gamma
\end{align}
```
↓↓↓

\begin{align}
    y &= ax + b \\\\\\\\
    \alpha \alpha &= \beta + \gamma
\end{align}

## 6. align*
```
$$
    \begin{align*}
        y = y(x,t) &= A e^{i\theta} \\
            &= A (\cos \theta + i \sin \theta) \\
            &= A (\cos(kx - \omega t) + i \sin(kx - \omega t)) \\
            &= A\cos(kx - \omega t) + i A\sin(kx - \omega t)  \\
            &= A\cos \Big(\frac{2\pi}{\lambda}x - \frac{2\pi v}{\lambda} t \Big) + i A\sin \Big(\frac{2\pi}{\lambda}x - \frac{2\pi v}{\lambda} t \Big)  \\
            &= A\cos \frac{2\pi}{\lambda} (x - v t) + i A\sin \frac{2\pi}{\lambda} (x - v t)
    \end{align*}
$$
```
↓↓↓

$$
    \begin{align*}
        y = y(x,t) &= A e^{i\theta} \\
            &= A (\cos \theta + i \sin \theta) \\
            &= A (\cos(kx - \omega t) + i \sin(kx - \omega t)) \\
            &= A\cos(kx - \omega t) + i A\sin(kx - \omega t)  \\
            &= A\cos \Big(\frac{2\pi}{\lambda}x - \frac{2\pi v}{\lambda} t \Big) + i A\sin \Big(\frac{2\pi}{\lambda}x - \frac{2\pi v}{\lambda} t \Big)  \\
            &= A\cos \frac{2\pi}{\lambda} (x - v t) + i A\sin \frac{2\pi}{\lambda} (x - v t)
    \end{align*}
$$


## 7. \mbox

```
$$
    \mbox{全平方和} &= \mbox{群間平方和 + 群内平方和（残差平方和）} \\
    &= 0.2204 + 0.3370  
$$
```
↓↓↓

$$
    \mbox{全平方和} &= \mbox{群間平方和 + 群内平方和（残差平方和）} \\
    &= 0.2204 + 0.3370  
$$


## 8. \mbox

```
$$
    \mbox{全平方和} = \mbox{群間平方和 + 群内平方和（残差平方和）} \\
    = 0.2204 + 0.3370  
$$
```
↓↓↓

$$
    \mbox{全平方和} &= \mbox{群間平方和 + 群内平方和（残差平方和）} \\
    &= 0.2204 + 0.3370  
$$




## 9. \mbox aligned
```
$$
\begin{aligned}
    \mbox{全平方和} &= \mbox{群間平方和 + 群内平方和（残差平方和）} \\
    &= 0.2204 + 0.3370  
\end{aligned}
$$
```
↓↓↓

$$
\begin{aligned}
    \mbox{全平方和} &= \mbox{群間平方和 + 群内平方和（残差平方和）} \\
    &= 0.2204 + 0.3370  
\end{aligned}
$$

## 10. \mbox aligned
```
\begin{aligned}
    \mbox{全平方和} &= \mbox{群間平方和 + 群内平方和（残差平方和）} \\\\\\
    &= 0.2204 + 0.3370  
\end{aligned}
```
↓↓↓

\begin{aligned}
    \mbox{全平方和} &= \mbox{群間平方和 + 群内平方和（残差平方和）} \\\\\\
    &= 0.2204 + 0.3370  
\end{aligned}


## 11. \mbox align
```
$$
    \begin{align}
        \mbox{全平方和} &= \mbox{群間平方和 + 群内平方和（残差平方和）} \\\\\\
        &= 0.2204 + 0.3370  
    \end{align}
$$
```
↓↓↓

$$
    \begin{align}
        \mbox{全平方和} &= \mbox{群間平方和 + 群内平方和（残差平方和）} \\\\\\
        &= 0.2204 + 0.3370  
    \end{align}
$$

## 12. \mbox align
```
\begin{align}
    \mbox{全平方和} &= \mbox{群間平方和 + 群内平方和（残差平方和）} \\\\\\
    &= 0.2204 + 0.3370  
\end{align}
```
↓↓↓

\begin{align}
    \mbox{全平方和} &= \mbox{群間平方和 + 群内平方和（残差平方和）} \\\\\\
    &= 0.2204 + 0.3370  
\end{align}

以上

